\documentclass{article}
\usepackage{amsmath}
\begin{document}
\title{Solution2}
\maketitle
\section{Problem}
In this senario, we consider the problem to find the most money-saving way to acquire the data inorder to achieve a satisfactory regret bound $R$. The objective function is in the form of a integral, which is not an easy problem of the classical optimization problem. Besides, to solve the very exact form of the budget . Thus we use the of the budget B as following
\begin{equation}
\sum_t c_t q_t \leq B \leq \sum_t Mq_t
\end{equation}
Thus what we have to do is to solve the optimization problem of the form
\begin{align}
&\min_{q_t} c_t\\
s.t. &\sum_t \frac{\nabla f_t^2}{q_t}\leq R\\
	&0\leq q_t \leq 1
\end{align}
\section{Solution}
Consider the convexity of the objective function, we give the Lagrangian
\begin{equation}
L=\sum_t c_t q_t -\lambda(-\sum_t\frac{\nabla f_t^2}{q_t}+R-\sum_t\mu_t(1-q_t))
\end{equation}
The optimal K-T condition of the problem \ref{} is 
\begin{align}
\frac{\partial L}{\partial q_t}=c_t-\lambda[\frac{\nabla f_t^2}{q_t^2}]-\mu_i=0
\end{align}
when $q_t=1$, we get $u_i\neq 0$, when $q_t\neq 1$, $\mu_i=0$, thus we have
\begin{equation}\label{BC:q}
q_t=\min\{1,\sqrt{\frac{\lambda}{c_t}}\nabla f_t\}
\end{equation}
According to our constraint condition
\begin{equation}
\sum_t \sqrt{\frac{c_t}{\lambda}}\nabla f_t\leq R
\end{equation}
\begin{align}
\sqrt{\lambda}&\geq\frac{\sum_t \sqrt{c_t}\nabla f_t}{R}\\
& =\frac{T}{R}(\frac{1}{T}\sum_t\sqrt{c_t}\nabla f_t)\\
& =\frac{T}{R}\theta
\end{align}
where we use $\theta$ to denote the term $\frac{1}{T}\sum_t\sqrt{c_t}\nabla f_t$.
Since \ref{BC:q} holds for $\forall c_t$, and $c_t$ is arbitrarily given.We may assume that the convoluted distribution function of the price mechanism is of the form 
\begin{equation}
F_t(c)=1-\sqrt{\frac{\lambda}{c}}\nabla f_t
\end{equation}
And the PDF is 
\begin{equation}
f(c)=\frac{1}{2}\sqrt{\lambda}{c^3}\nabla f_t
\end{equation}
\section{Analysis}
Now we can make a relatively more precise estimate the budget $B$
\begin{align}
B&=\sum_t\int_{c_t}^Mcf(c)dc\\
&=\sum_t\int_{c_t}^M\frac{1}{2}\sqrt{\frac{\lambda}{c}}\nabla f_t dc\\
&=\sum_t\sqrt{\lambda}\nabla f_t(\sqrt){M}-\sqrt{c_t})\\
&=\frac{T^2}{R}(\frac{1}{T}\sum_t\sqrt{c_t}\nabla f_t)(\sum_t \frac{1}{T}\nabla f_t(\sqrt{M}-\sqrt{c-t}))\\
&=\frac{T^2}{R}\theta\varphi
\end{align}
where $\varphi=\sum_t\frac{1}{T}\nabla f_t(\sqrt{M}-\sqrt{c_t})$




\end{document}
